Implements the message header deserialization
Implements https://code.amazon.com/packages/TmpAWSEncryptionSDKSpec/blobs/mainline/--/message-header.md

There are some TODOs left in the code. Especially for parts of the code which are weakly specified or not yet specified, or for which I could not find the specification. The message header especially is not clearly specified yet.

src/Util/StandardLibrary.dfy
@@ -4,15 +4,100 @@ module {:extern "STL"} StandardLibrary {
   newtype byte = x | 0 <= x < 256
   type uint8 = byte
 
+  newtype uint16 = x | 0 <= x < 0x1_0000
+  const UINT16_MAX := 0x1_0000 - 1
+
   newtype int32 = x | -0x8000_0000 <= x < 0x8000_0000
 
   newtype uint32 = x | 0 <= x < 0x1_0000_0000
+  const UINT32_MAX := 0x1_0000_0000 - 1
+
+  newtype uint64 = x | 0 <= x < 0x1_0000_0000_0000_0000
 
   function Fill<T>(value: T, n: nat): seq<T>
     ensures |Fill(value, n)| == n
     ensures forall i :: 0 <= i < n ==> Fill(value, n)[i] == value
   {
     if n > 0 then [value] + Fill(value, n-1) else []
+  }
+
+  function method deser_uint16_from_array (p : array<byte>) : uint16
+    reads p
+    requires p.Length == 2
+  {
+    var x1 := p[0] as int * 256;
+    assert x1 <= 256 * 256;
+    var x := x1 + p[1] as int;
+    assert x <= UINT16_MAX;
+    x as uint16
+  }
+
+  function method deser_uint32_from_array (p : array<byte>) : uint32
+    reads p
+    requires p.Length == 4
+  {
+    // 2^24 = 0x100_0000
+    var x3 :=      p[0] as int * 0x100_0000;
+    // 2^16 = 0x1_0000
+    var x2 := x3 + p[1] as int * 0x1_0000;
+    // 2^8 = 0x100
+    var x1 := x2 + p[2] as int * 0x100;
+    // 2^0 = 0x1
+    var  x := x1 + p[3] as int;
+    assert x <= UINT32_MAX;
+    x as uint32
+  }
+
+  datatype Either<S,T> = Left(left: S) | Right(right: T)
+
+  datatype Error = IOError(m: string) | DeserializationError(m: string)
+
+  type Result<T> = Either<T, Error>
+
+  method values<A,B>(m: map<A,B>) returns (vals: seq<B>)
+    ensures |vals| == |m|
+  {
+    var keys := m.Keys;
+    vals := [];
+    while keys != {}
+      decreases keys
+      invariant |keys| + |vals| == |m.Keys|
+    {
+      var a :| a in keys;
+      keys := keys - {a};
+      vals := vals + [m[a]];
+    }
+  }
+
+  predicate method ltByte(a: byte, b: byte) { a < b }
+  predicate method ltNat (a: nat,  b: nat)  { a < b }
+  predicate method ltInt (a: int,  b: int)  { a < b }
+  
+  predicate method lexCmpArrays<T(==)>(a : array<T>, b : array<T>, lt: (T, T) -> bool)
+      reads a, b
+  {
+      a.Length == 0 || (b.Length != 0 && lexCmpArraysNonEmpty(a, b, 0, lt))
+  }
+
+  predicate method lexCmpArraysNonEmpty<T(==)>(a : array<T>, b : array<T>, i: nat, lt: (T, T) -> bool)
+      requires i < a.Length
+      requires i < b.Length
+      requires forall j: nat :: j < i ==> a[j] == b[j]
+      decreases a.Length - i
+      reads a, b
+  {
+      if a[i] != b[i] 
+      then lt(a[i], b[i])
+      else 
+          if i+1 < a.Length && i+1 < b.Length
+          then lexCmpArraysNonEmpty(a, b, i+1, lt)
+          else 
+              if i+1 == a.Length && i+1 < b.Length
+              then true
+              else
+                  if i+1 < a.Length && i+1 == b.Length
+                  then false
+                  else true // i+1 == a.Length && i+1 == b.Length, i.e. a == b
   }
 
 }
