src/SDK/AlgorithmSuite.dfy
@@ -1,0 +1,38 @@
+include "../Crypto/All.dfy"
+include "../Crypto/Cipher.dfy"
+include "../Crypto/Digests.dfy"
+include "../Util/StandardLibrary.dfy"
+
+module AlgorithmSuite {
+
+  import opened Cipher
+  import Digests
+  import S = Signature
+  import opened StandardLibrary
+
+  newtype ID = x | 0 <= x < 0x1_0000
+  const AES_256_GCM_IV12_AUTH16_KDSHA384_SIGEC384 : ID := 0x0378
+  const AES_192_GCM_IV12_AUTH16_KDSHA384_SIGEC384 : ID := 0x0346
+  const AES_128_GCM_IV12_AUTH16_KDSHA256_SIGEC256 : ID := 0x0214
+  const AES_256_GCM_IV12_AUTH16_KDSHA256_SIGNONE  : ID := 0x0178
+  const AES_192_GCM_IV12_AUTH16_KDSHA256_SIGNONE  : ID := 0x0146
+  const AES_128_GCM_IV12_AUTH16_KDSHA256_SIGNONE  : ID := 0x0114
+  const AES_256_GCM_IV12_AUTH16_KDNONE_SIGNONE    : ID := 0x0078
+  const AES_192_GCM_IV12_AUTH16_KDNONE_SIGNONE    : ID := 0x0046
+  const AES_128_GCM_IV12_AUTH16_KDNONE_SIGNONE    : ID := 0x0014
+
+  datatype AlgSuite = AlgSuite(params : Cipher.CipherParams, hkdf : Digests.HMAC_ALGORITHM, sign : Option<S.ECDSAParams>)
+
+  const Suite := map [
+    AES_256_GCM_IV12_AUTH16_KDSHA384_SIGEC384 := AlgSuite(CipherParams(AES256, 16, 12), Digests.HmacSHA384, Some(S.ECDSA_P384)),
+    AES_192_GCM_IV12_AUTH16_KDSHA384_SIGEC384 := AlgSuite(CipherParams(AES192, 16, 12), Digests.HmacSHA384, Some(S.ECDSA_P384)),
+    AES_128_GCM_IV12_AUTH16_KDSHA256_SIGEC256 := AlgSuite(CipherParams(AES128, 16, 12), Digests.HmacSHA256, Some(S.ECDSA_P256)),
+    AES_256_GCM_IV12_AUTH16_KDSHA256_SIGNONE  := AlgSuite(CipherParams(AES256, 16, 12), Digests.HmacSHA256, None),
+    AES_192_GCM_IV12_AUTH16_KDSHA256_SIGNONE  := AlgSuite(CipherParams(AES192, 16, 12), Digests.HmacSHA256, None),
+    AES_128_GCM_IV12_AUTH16_KDSHA256_SIGNONE  := AlgSuite(CipherParams(AES128, 16, 12), Digests.HmacSHA256, None),
+    AES_256_GCM_IV12_AUTH16_KDNONE_SIGNONE    := AlgSuite(CipherParams(AES256, 16, 12), Digests.HmacNOSHA,  None),
+    AES_192_GCM_IV12_AUTH16_KDNONE_SIGNONE    := AlgSuite(CipherParams(AES192, 16, 12), Digests.HmacNOSHA,  None),
+    AES_128_GCM_IV12_AUTH16_KDNONE_SIGNONE    := AlgSuite(CipherParams(AES128, 16, 12), Digests.HmacNOSHA,  None)
+  ]
+
+}
